Merge iris/base_logic/lib/mono_map and iris/base_logic/lib/mono_map_.

theories/iris/base_logic/lib/mono_map.v
@@ -12,12 +12,15 @@ From zebre.iris Require Import
 From zebre Require Import
   options.
 
+#[local] Definition mono_map_UR K V `{Countable K} :=
+  authUR $ gmapUR K $ agreeR $ leibnizO V.
+
 Class MonoMapG Σ K V `{Countable K} := {
-  #[local] mono_map_G_inG :: inG Σ (authUR $ gmapUR K $ agreeR V) ;
+  #[local] mono_map_G_inG :: inG Σ (mono_map_UR K V) ;
 }.
 
 Definition mono_map_Σ K V `{Countable K} := #[
-  GFunctor (authUR $ gmapUR K $ agreeR V)
+  GFunctor (mono_map_UR K V)
 ].
 #[global] Instance subG_mono_map_Σ Σ K V `{Countable K} :
   subG (mono_map_Σ K V) Σ →
@@ -29,49 +32,61 @@ Qed.
 Section mono_map_G.
   Context `{mono_map_G : MonoMapG Σ K V}.
 
-  Definition mono_map_auth γ σ :=
-    @own _ _ mono_map_G_inG γ (● (to_agree <$> σ)).
+  Implicit Types m : gmap K V.
+
+  #[local] Canonical V_O :=
+    leibnizO V.
+
+  Definition mono_map_auth γ m :=
+    @own _ _ mono_map_G_inG γ (● (to_agree <$> m)).
+  Definition mono_map_lb γ m :=
+    @own _ _ mono_map_G_inG γ (◯ (to_agree <$> m)).
   Definition mono_map_elem γ i v :=
-    @own _ _ mono_map_G_inG γ (◯ {[i := to_agree v]}).
+    mono_map_lb γ {[i := v]}.
 
-  #[global] Instance mono_map_elem_timeless γ i v :
-    Discrete v →
-    Timeless (mono_map_elem γ i v).
+  #[global] Instance mono_map_auth_timeless γ m :
+    Timeless (mono_map_auth γ m).
   Proof.
     apply _.
   Qed.
-  #[global] Instance mono_map_elem_persistent γ i v :
-    Persistent (mono_map_elem γ i v).
+  #[global] Instance mono_map_lb_timeless γ m :
+    Timeless (mono_map_lb γ m).
+  Proof.
+    apply _.
+  Qed.
+  #[global] Instance mono_map_lb_persistent γ m :
+    Persistent (mono_map_lb γ m).
   Proof.
     apply _.
   Qed.
 
-  Lemma mono_map_alloc α :
+  Lemma mono_map_alloc m :
     ⊢ |==>
       ∃ γ,
-      mono_map_auth γ α.
+      mono_map_auth γ m.
   Proof.
     iApply own_alloc. apply auth_auth_valid.
-    intros i. rewrite lookup_fmap. by destruct (α !! i).
+    intros i. rewrite lookup_fmap. by destruct (m !! i).
   Qed.
 
-  Lemma mono_map_insert γ σ i v :
-    σ !! i = None →
-    mono_map_auth γ σ ⊢ |==>
-      mono_map_auth γ (<[i:=v]> σ) ∗
-      mono_map_elem γ i v.
+  Lemma mono_map_lb_get γ m :
+    mono_map_auth γ m ⊢ |==>
+      mono_map_auth γ m ∗
+      mono_map_lb γ m.
   Proof.
-    iIntros (Hi) "?". rewrite /mono_map_elem /mono_map_auth.
-    rewrite -own_op. iApply (own_update with "[$]").
-    apply auth_update_alloc. rewrite fmap_insert. apply alloc_singleton_local_update.
-    { rewrite lookup_fmap Hi //. }
-    done.
+    rewrite /mono_map_auth /mono_map_lb -own_op.
+    iApply own_update. apply auth_update_alloc.
+    apply local_update_unital. intros n z Hv Hz.
+    rewrite mixin_ucmra_unit_left_id in Hz. apply gmap_ucmra_mixin.
+    split. eauto.
+    rewrite -Hz gmap_op.
+    intros l. rewrite lookup_merge lookup_fmap.
+    destruct (m !! l); last done. simpl. rewrite -Some_op agree_idemp //.
   Qed.
-
-  Lemma mono_map_extract γ σ i v :
-    σ !! i = Some v ->
-    mono_map_auth γ σ ⊢ |==>
-      mono_map_auth γ σ ∗
+  Lemma mono_map_elem_get {γ m} i v :
+    m !! i = Some v →
+    mono_map_auth γ m ⊢ |==>
+      mono_map_auth γ m ∗
       mono_map_elem γ i v.
   Proof.
     iIntros (Hi) "He". rewrite /mono_map_elem /mono_map_auth.
@@ -81,33 +96,63 @@ Section mono_map_G.
     rewrite mixin_ucmra_unit_left_id in Hz; first apply gmap_ucmra_mixin.
     split. eauto.
     rewrite -Hz.
-    rewrite -{2}(insert_id σ i v) // fmap_insert -insert_op.
+    rewrite -{2}(insert_id m i v) // fmap_insert map_fmap_singleton -insert_op.
     rewrite agree_idemp left_id // insert_id //.
     rewrite lookup_fmap Hi //.
   Qed.
 
-  Lemma mono_map_lookup `{!LeibnizEquiv V} `{OfeDiscrete V} γ σ i v :
-    mono_map_auth γ σ -∗
-    mono_map_elem γ i v -∗
-    ⌜σ !! i = Some v⌝.
+  Lemma mono_map_insert {γ m} i v :
+    m !! i = None →
+    mono_map_auth γ m ⊢ |==>
+    mono_map_auth γ (<[i := v]> m).
+  Proof.
+    iIntros (Hi) "?". iApply (own_update with "[$]").
+    rewrite fmap_insert. apply auth_update_auth with (b':={[i:=to_agree v]}).
+    apply (@alloc_singleton_local_update K _ _ (agreeR $ leibnizO V) (to_agree <$> m) i (to_agree v)).
+    { rewrite lookup_fmap Hi //. }
+    done.
+  Qed.
+  Lemma mono_map_insert' {γ m} i v :
+    m !! i = None →
+    mono_map_auth γ m ⊢ |==>
+      mono_map_auth γ (<[i:=v]> m) ∗
+      mono_map_elem γ i v.
+  Proof.
+    iIntros "%Hlookup Hauth".
+    iMod (mono_map_insert with "Hauth") as "Hauth"; first done.
+    iApply (mono_map_elem_get with "Hauth"); first rewrite lookup_insert //.
+  Qed.
+
+  Lemma mono_map_lb_valid γ m1 m2 :
+    mono_map_auth γ m1 -∗
+    mono_map_lb γ m2 -∗
+    ⌜m2 ⊆ m1⌝.
   Proof.
     iIntros "Ha Hf".
     iDestruct (own_valid_2 with "Ha Hf") as "%Hv".
     iPureIntro.
     apply auth_both_valid_discrete in Hv. destruct Hv as (Hv&_).
-    apply singleton_included_l in Hv. destruct Hv as (y,(Hv1&Hv2)).
-    rewrite lookup_fmap in Hv1.
-    destruct (σ !! i) as [w|] eqn:Hw.
-    2:{ exfalso. inversion Hv1. }
-    simpl in Hv1. rewrite -Hv1 in Hv2.
-    assert (v ≡ w ) as Hv.
-    { apply Some_included in Hv2. destruct Hv2 as [Hv2|Hv2].
-      - by apply to_agree_inj in Hv2.
-      - by apply to_agree_included in Hv2.
+    intros i. eapply lookup_included with (i:=i) in Hv.
+    rewrite !lookup_fmap in Hv.
+    destruct (m1!!i),(m2!!i); try done; simpl in *.
+    { apply Some_included in Hv. simpl. eapply (@leibniz_equiv (leibnizO V)). apply _.
+      destruct Hv as [Hv|Hv].
+      - by apply to_agree_inj.
+      - by apply to_agree_included.
+    } {
+      apply Some_included_is_Some in Hv. by inversion Hv.
     }
-    apply leibniz_equiv in Hv. naive_solver.
+  Qed.
+  Lemma mono_map_elem_valid γ m i v :
+    mono_map_auth γ m -∗
+    mono_map_elem γ i v -∗
+    ⌜m !! i = Some v⌝.
+  Proof.
+    iIntros "Hauth Helem".
+    iDestruct (mono_map_lb_valid with "Hauth Helem") as %?%map_singleton_subseteq_l.
+    iSteps.
   Qed.
 End mono_map_G.
 
 #[global] Opaque mono_map_auth.
-#[global] Opaque mono_map_elem.
+#[global] Opaque mono_map_lb.
